etch4/Etch/Verification/Semantics/OldBSearch.lean
@@ -7,32 +7,33 @@ import Mathlib.Init.Algebra.Order
 namespace Etch.Verification
 open Streams
 
-variable (α : Type) [Inhabited α] [LinearOrder α]
+
 /-- A type representing a state in a binary search stream. -/
-  structure BSearchState where
+  structure BSearchState (α : Type) where
     is     : List α -- The array of indices
-    h_sorted : List.Sorted (. ≤ .) is
-    h_nonempty : is ≠ [] 
     target : α -- The item to find
     currLo : ℕ  -- The lower boundary index for the subarray under consideration
     currHi : ℕ -- The upper boundary index for the subarray under consideration
     -- found  : Bool -- Represents whether the current search was successful
   deriving Repr
 
-  /-- Computes midpoint of two array indices. -/
-def mid (lo hi : ℕ) : ℕ := lo + (hi - lo) / 2  
+    /-- Computes midpoint of two array indices. -/
+  def mid (lo hi : ℕ) : ℕ := lo + (hi - lo) / 2  
 
-def BSearchState.found (q : BSearchState α) : Prop := (q.is[mid q.currLo q.currHi]! = q.target)
-def BSearchState.arrInd  (q : BSearchState α) :  ℕ := mid q.currLo q.currHi
+  def BSearchState.found [Inhabited α] [Preorder α] (q : BSearchState α) : Prop := (q.is[mid q.currLo q.currHi]! = q.target)
+  def BSearchState.arrInd  (q : BSearchState α) :  ℕ := mid q.currLo q.currHi
 
-abbrev BSearchState.done (q : BSearchState α) : Prop := ¬(q.currLo <= q.currHi ∧ q.currHi ≠ 0 ∧ ¬(q.is[mid q.currLo q.currHi]! = q.target))
+def BSearchState.done [Inhabited α] (q : BSearchState α) : Prop := ¬(q.currLo <= q.currHi ∧ ¬(q.is[mid q.currLo q.currHi]! = q.target))
 
+
+variable [Inhabited α] 
+[LinearOrder α]
   def skip' (q : BSearchState α) (i : α) (r : Bool): BSearchState α :=
     if i > q.target then -- Reset search
       {q with target := i, currHi := q.is.length - 1}
       -- equivalent to ⟨q.is, i, q.currLo, q.is.length - 1⟩
     else if i < q.target then q -- No-op
-    else if ¬q.done then  -- Continue search. Added q.currHi ≠ 0 to avoid infinite loop due to Nat bottoming out
+    else if q.currLo <= q.currHi ∧ q.currHi ≠ 0 ∧ ¬(q.is[mid q.currLo q.currHi]! = q.target) then  -- Continue search. Added q.currHi ≠ 0 to avoid infinite loop due to Nat bottoming out
       if q.target < q.is[q.arrInd]! then 
         {q with currHi := q.arrInd - 1}
       else if q.target > q.is[q.arrInd]! then
@@ -45,10 +46,13 @@ abbrev BSearchState.done (q : BSearchState α) : Prop := ¬(q.currLo <= q.currHi
            target := q.is[q.arrInd + 1]'h
            currLo := q.arrInd + 1,
            currHi := q.arrInd + 1}
-        else {q with currLo := q.arrInd + 1} -- aha, this case is problematic perhaps. unless we add the assumption that the next state is valid
+        else {q with currLo := q.arrInd + 1}
       else
         q
 
+variable (α)
+variable [Inhabited α] 
+[LinearOrder α]
 
  /-- A stream representing a binary search on an array. -/
 def bSearch : Stream α ℕ where
@@ -56,7 +60,7 @@ def bSearch : Stream α ℕ where
   index q _ := q.target
   value q _ := q.arrInd
   ready q := q.found
-  skip q _ prod := skip' α q prod.fst prod.snd
+  skip q _ prod := skip' q prod.fst prod.snd
   valid q := q.arrInd < q.is.length
 
 def inv_conj (q : BSearchState α) : Prop :=
@@ -71,11 +75,21 @@ theorem inv_init (q : BSearchState α) : q.currLo = 0 ∧ q.currHi = q.is.length
   rw [list_eq_cons_head_tail h_nonempty] at h_sorted
   apply And.intro
   . sorry -- I think I want List.rel_of_sorted_cons
+
+
+    -- exact List.rel_of_sorted_cons h_sorted q.target h_mem -- what's an easy way to say this list is nonempty
   . sorry
 
+    
+    -- why is lean being weird
 
 
 theorem invariant (q : BSearchState α) : inv_conj α q := sorry -- this shouldn't actually be a universal i think, just for all q in the transition system
+
+  
+
+  
+
 
 theorem bsearch_correctness (q : BSearchState α) : List.Sorted (. ≤ .) q.is → q.is ≠ [] → q.done → List.Mem q.target q.is → q.is[q.arrInd]! = q.target := by
   intros sorted nonempty done mem
@@ -117,6 +131,16 @@ theorem bsearch_correctness' (q : BSearchState α) : List.Sorted (. ≤ .) q.is 
     
 
 
+
+
+
+
+
+
+
+
+
+
 theorem bsearch_is_mono : (bSearch α).IsMonotonic := by
   intros q hq i
   unfold Stream.index'
@@ -128,18 +152,15 @@ theorem bsearch_is_mono : (bSearch α).IsMonotonic := by
     repeat first | rfl | split_ifs
     . simp only [BSearchState.arrInd, mid]
       have tgt_exists_or_not : List.Mem q.target q.is ∨ ¬List.Mem q.target q.is := or_not
-      rename ¬BSearchState.done α q => h_not_done
+      have h_sorted : List.Sorted (. ≤ .) q.is := by sorry
+      rename ¬(q.currLo ≤ q.currHi ∧ q.currHi ≠ 0 ∧ ¬q.is[mid q.currLo q.currHi]! = q.target) => h_done
       cases tgt_exists_or_not
       . rename List.Mem q.target q.is => h_tgt_exists
-        have : (q.done → List.Mem q.target q.is → q.is[q.arrInd]! = q.target) := bsearch_correctness α q q.h_sorted q.h_nonempty   -- bsearch_correctness α q h_sorted h_done h_tgt_exists
+        have : q.is[q.arrInd]! = q.target := sorry -- bsearch_correctness α q h_sorted h_done h_tgt_exists
         simp only [BSearchState.arrInd, mid] at this
         rw [←this]
-         -- the new goal follows from the fact that it's sorted, but idk how to show it yet
-        have le_succ (j : Nat) : q.is[j]! ≤ q.is[j + 1]'(by sorry) := sorry -- also it's strange that one of these needs an indexing proof but the other none
-        exact le_succ (q.currLo + (q.currHi - q.currLo) / 2)
-        sorry -- contradiction, i think. but why is this a goal?
-        -- anyway, maybe rewrite h_not_done with demorgan's laws and work by cases
-        assumption -- again, not sure why this is a goal
+         -- the new goal follows from the fact that it's sorted, but idk
+        sorry
       . sorry -- Is it enough to show that q.is[q.currLo + (q.currHi - q.currLo) / 2] ≤ q.is[q.currLo + (q.currHi - q.currLo) / 2 + 1]
     repeat rfl
   . exact le_top
@@ -164,9 +185,7 @@ theorem bsearch_is_strict_mono : (bSearch α).IsStrictMono := by
       unfold Stream.toOrder at hi
       unfold bSearch at hi
       simp only [Bool.decide_coe] at hi
-      unfold BSearchState.found at hi
       rename i.fst < q.target => i_lt_tgt
-      -- Ok so we wrote a proof by contradiction here but it got broken with some refactoring. That's ok. The logic still works I think
       have coe_hi : toLex (q.target, q.found) ≤ toLex i := hi 
       have : (q.target, q.found).fst < i.fst ∨ (q.target, q.found).fst = i.fst ∧ (q.target, q.found).snd ≤ i.snd :=
        (Prod.Lex.le_iff (q.target, q.found) i).mp coe_hi
