etch4/Etch/Verification/Semantics/StartingFromScratchJacobs.lean
@@ -1,0 +1,74 @@
+import Etch.Verification.Semantics.SkipStream
+import Etch.Basic
+import Mathlib.Init.Algebra.Order
+
+/- This file is an attempt to prove that the BSearch stream is strictly lawful. -/
+
+namespace Etch.Verification
+open Streams
+
+
+variable (ι : Type) [Inhabited ι] [LinearOrder ι] [OrderTop ι] [OrderBot ι]
+
+structure Arr where
+  xs : List ι
+
+def Arr.get (arr : Arr ι) (i : Int) : ι :=
+  match i with
+  | Int.ofNat n => if h : n < arr.xs.length then  arr.xs[n]'h else ⊤
+  | _ => ⊥
+
+
+variable (is : Arr ι) (mid : ℤ → ℤ → ℤ)
+/-- A type representing a state in a binary search stream. -/
+structure BSearchState  where
+  left : ℤ
+  right : ℤ
+
+-- (is : Arr ι) (mid : ℤ → ℤ → ℤ) Don't use as parametesrs. well i know we'd said this, but I think we're fundamentally doing a different search if not
+
+
+
+abbrev BSearchState.loopTest (q : BSearchState) : Prop := q.right - q.left > 1
+
+/--- Carries out a step of binary search. -/
+def bSearchStep (q : BSearchState) (p : ℤ → Prop) [DecidablePred p]:= -- incrementally designing
+  if q.loopTest then
+    let m : ℤ := mid q.left q.right
+    if p m then {q with right := m} else {q with left := m}
+  else q -- extract the lower and upper from this
+
+
+
+-- Need to be careful here. Need to avoid changing predicate or middle function in the middle of a search
+
+theorem t (q : BSearchState) (p : ℤ → Prop) : ¬p q.left ∧ p q.right ∧ ¬q.loopTest → q.right = q.left + 1 ∧  ¬p q.left ∧ p q.right := by
+intro h
+apply And.intro
+. unfold BSearchState.loopTest at h
+  sorry
+  -- h sort of encodes the goal. We got here by calling mid, and mid is strictly between. how to show lean? DO on paper first I guess
+. exact And.intro h.left h.right.left
+
+
+ /-- A stream representing a binary search on an array. -/
+def bSearch (is : Arr ι) : Stream ι (ℤ × ℤ)  where
+  σ := BSearchState
+  index q _ := is.get ι q.left
+  value q _ := (q.left, q.right)
+  ready q := ¬q.loopTest
+  skip q _ prod := sorry -- skip' ι q prod.fst prod.snd
+  valid q := sorry -- q.arrInd < is.length
+
+
+/- I think when we reset the search we should start at the old left.
+    But how do we keep monotonicity with pairs? OH, well have ordering lexicographic hwere if first part of pair greater than whole thing greater. Not eq
+
+   -/
+
+/- How do I enforce stream properties?
+I guess if the pred were something like x <= a, then we would have to go to x <= the next thing in the array
+Which I think I can do in my skip implementation but ignore in bsearchStep
+
+That means BSearchState can't be parameterized in terms of the predicate. But I think I can have variable (is : Arr ι) (mid : ℤ → ℤ → ℤ) be params
+-/
